proofs/GoLeanProofs.lean
@@ -32,6 +32,7 @@ import GoLeanProofs.Specs.AutomationTargets
 import GoLeanProofs.Specs.GoldenQuorumThree
 import GoLeanProofs.Specs.GoldenQuorumAll
 import GoLeanProofs.Specs.TotalPins
+import GoLeanProofs.Specs.GoldenForkJoin
 import GoLeanProofs.NegativeSpecs
 
 /-!
